examples/ip: Prove correctness of lowered Gallina ip_checksum

src/Rupicola/Examples/Net/IPChecksum/Impl.v
@@ -38,3 +38,332 @@ Definition ip_checksum_impl (bs: list byte) : word :=
 
   let/n chk16 := (~w chk16) &w 0xffff in
   chk16.
+
+Section Properties.
+  Lemma Z_div_eucl_unique a b q q' r r':
+    0 <= r < b \/ b < r <= 0 ->
+    0 <= r' < b \/ b < r' <= 0 ->
+    a = b * q + r ->
+    a = b * q' + r' ->
+    (q = q' /\ r = r').
+  Proof.
+    intros Hr Hr' Hq Hq';
+      erewrite (Z.div_unique a b q r Hr Hq);
+      erewrite (Z.div_unique a b q' r' Hr' Hq');
+      erewrite (Z.mod_unique a b q r Hr Hq);
+      erewrite (Z.mod_unique a b q' r' Hr' Hq');
+      split; reflexivity.
+  Qed.
+
+  Lemma Nat2Z_inj_div_mod a b:
+    Z.of_nat (a / b) = Z.of_nat a / Z.of_nat b /\
+    Z.of_nat (a mod b) = Z.of_nat a mod Z.of_nat b.
+  Proof.
+    destruct (Nat.eq_dec b 0) as [->|].
+    - destruct a; split; reflexivity.
+    - pose (q := (a / b)%nat).
+      pose (r := (a mod b)%nat).
+      assert (a = b * q + r)%nat as Hnat by (apply Nat_mod_eq'; lia).
+      pose (zq := Z.of_nat a / Z.of_nat b).
+      pose (zr := Z.of_nat a mod Z.of_nat b).
+      assert (Z.of_nat a = Z.of_nat b * zq + zr) as Hz by (apply Z_mod_eq'; lia).
+      apply (f_equal Z.of_nat) in Hnat.
+      rewrite Nat2Z.inj_add, Nat2Z.inj_mul in Hnat.
+      pose proof Nat.mod_bound_pos a b ltac:(lia) ltac:(lia).
+      pose proof Z.mod_bound_or (Z.of_nat a) (Z.of_nat b).
+      eapply Z_div_eucl_unique; try eassumption.
+      all: try lia.
+  Qed.
+
+  Lemma Nat2Z_inj_div a b:
+    Z.of_nat (a / b) = Z.of_nat a / Z.of_nat b.
+  Proof. apply (Nat2Z_inj_div_mod a b). Qed.
+
+  Lemma Nat2Z_inj_mod a b:
+    Z.of_nat (a mod b) = Z.of_nat a mod Z.of_nat b.
+  Proof. apply (Nat2Z_inj_div_mod a b). Qed.
+
+  Lemma z_range_add from len:
+    z_range from (from + len) = z_range' from (Z.to_nat len).
+  Proof. unfold z_range; do 2 f_equal; lia. Qed.
+
+  Lemma Nat2Z_inj_odd : forall n,
+    Z.odd (Z.of_nat n) = Nat.odd n.
+  Proof.
+    apply Nat.pair_induction.
+    - intros ?? ->; reflexivity.
+    - reflexivity.
+    - reflexivity.
+    - intros; rewrite !Nat2Z.inj_succ, Z.odd_succ_succ. eassumption.
+  Qed.
+
+  Lemma Natmod_odd: forall a : nat,
+      (a mod 2 = if Nat.odd a then 1 else 0)%nat.
+  Proof.
+    apply Nat.pair_induction.
+    - intros ?? ->; reflexivity.
+    - reflexivity.
+    - reflexivity.
+    - intros.
+      replace (S (S n)) with (n + 1 * 2)%nat at 1 by lia.
+      rewrite Nat.mod_add by lia.
+      eassumption.
+  Qed.
+
+  Lemma Natodd_mod : forall a : nat,
+      (Nat.odd a = negb (a mod 2 =? 0))%nat.
+  Proof.
+    intros; rewrite Natmod_odd.
+    destruct Nat.odd; reflexivity.
+  Qed.
+
+  Lemma nat_div2_spec n:
+    ((n = 2 * (n / 2) /\ n mod 2 = 0) \/
+     (n = 2 * (n / 2) + 1 /\ n mod 2 = 1))%nat.
+  Proof.
+    pose proof Nat.mod_bound_pos n 2 ltac:(lia) ltac:(lia).
+    pose proof (Nat_mod_eq' n 2 ltac:(lia)).
+    assert ((n mod 2 = 0) \/ (n mod 2 = 1))%nat as [Heq | Heq] by lia;
+      rewrite Heq in *; lia.
+  Qed.
+
+  Lemma ranged_for_all_nd_combine2 {A} (f: A -> byte -> byte -> A) (bs: list byte) n acc:
+    (n >= length bs)%nat ->
+    (let acc := ranged_for_all_nd
+                 0 (Z.of_nat n / 2)
+                 (fun acc idx =>
+                    f acc
+                      (ListArray.get bs (2 * idx))
+                      (ListArray.get bs (2 * idx + 1)))
+                 acc in
+     if Z.odd (Z.of_nat n) then f acc (ListArray.get bs (Z.of_nat n - 1)) default
+     else acc) =
+      (ranged_for_all_nd
+         0 (Z.of_nat (Nat.div_up n 2))
+         (fun acc idx =>
+            f acc
+              (ListArray.get bs (2 * idx))
+              (ListArray.get bs (2 * idx + 1)))
+         acc).
+  Proof.
+    intros.
+    rewrite div_up_eqn.
+    rewrite Nat2Z.inj_add.
+    rewrite <- !fold_left_as_ranged_for_all_nd.
+    rewrite (z_range_app 0 (Z.of_nat (n / 2)) (_ + _)) by lia.
+    rewrite fold_left_app.
+    rewrite Nat2Z_inj_div.
+    set (fold_left _ (z_range 0 _) _) as prefix.
+    rewrite z_range_add, Nat2Z.id.
+    rewrite Nat2Z_inj_odd, Natodd_mod.
+    destruct (nat_div2_spec n) as [(Heq, ->) | (Heq, ->)];
+      cbn [Nat.eqb negb z_range' List.fold_left].
+    - reflexivity.
+    - rewrite <- Nat2Z_inj_div.
+      f_equal.
+      + f_equal; lia.
+      + unfold ListArray.get, cast, Convertible_Z_nat; rewrite nth_overflow by lia;
+          reflexivity.
+  Qed.
+
+  Lemma fold_left_push_fn {A A' B}
+        (f: A -> B -> A)
+        (f': A' -> B -> A')
+        (g: A -> A')
+        (P: A -> Prop):
+    forall (l: list B),
+      (forall a0 a, List.In a l -> P a0 -> P (f a0 a)) ->
+      (forall a0 a, List.In a l -> P a0 -> g (f a0 a) = f' (g a0) a) ->
+      forall (a0: A),
+        P a0 ->
+        g (fold_left f l a0) = fold_left f' l (g a0).
+  Proof.
+    induction l; simpl; intros HP Hg a0 Pa0.
+    - reflexivity.
+    - rewrite IHl, Hg; eauto.
+  Qed.
+
+  Definition word_onec_add16 w1 w2 :=
+    let sum := word.add (word := word) w1 w2 in
+    word.add (word.and sum (word.of_Z 65535)) (word.sru sum (word.of_Z 16)).
+
+  Lemma word_unsigned_onec_add w1 w2:
+    let z1 := word.unsigned w1 in
+    let z2 := word.unsigned w2 in
+    0 <= z1 < 2 ^ 16 ->
+    0 <= z2 < 2 ^ 16 ->
+    word.unsigned (word_onec_add16 w1 w2) =
+    onec_add16 z1 z2.
+  Proof.
+    intros; unfold onec_add16, word_onec_add16.
+    pose proof Z_land_leq_right (z1 + z2) 0xffff ltac:(lia) ltac:(lia).
+    pose proof Z_shiftr_add_carry 16 16 z1 z2 ltac:(lia) ltac:(lia) ltac:(lia).
+
+    all: subst z1 z2.
+    repeat (rewrite ?word.unsigned_add, ?word.unsigned_and_nowrap;
+            rewrite ?word.unsigned_sru_shamtZ by lia;
+            rewrite ?word.unsigned_of_Z_nowrap, ?word.Z_land_wrap_l by lia).
+    rewrite_strat (repeat (innermost word.wrap_small)).
+
+    all: lia.
+  Qed.
+
+  Lemma word_unsigned_onec_add' z1 z2:
+    0 <= z1 < 2 ^ 16 ->
+    0 <= z2 < 2 ^ 16 ->
+    onec_add16 z1 z2 =
+    word.unsigned (word_onec_add16 (word.of_Z z1) (word.of_Z z2)).
+  Proof.
+    intros; rewrite word_unsigned_onec_add;
+      rewrite !word.unsigned_of_Z_nowrap; try lia.
+  Qed.
+
+  Lemma word_morph_onec_add z1 z2:
+    0 <= z1 < 2 ^ 16 ->
+    0 <= z2 < 2 ^ 16 ->
+    word.of_Z (onec_add16 z1 z2) = word_onec_add16 (word.of_Z z1) (word.of_Z z2).
+  Proof.
+    pose proof onec_add16_loose_bounds z1 z2.
+    intros; apply word.unsigned_inj;
+      rewrite word_unsigned_onec_add;
+      rewrite !word.unsigned_of_Z_nowrap; try lia.
+  Qed.
+
+  Lemma nth_chunk {A} k (Hk: (k <> 0)%nat) (bs: list A) i d
+        (Hi : (i < Nat.div_up (length bs) k)%nat) :
+    nth i (chunk k bs) d = firstn k (skipn (i*k) bs).
+  Proof.
+    pose proof nth_error_chunk k Hk bs i Hi as Hn.
+    eapply nth_error_nth in Hn; eassumption.
+  Qed.
+
+  Lemma nth_seq len: forall i start d,
+    (i < len)%nat ->
+    nth i (seq start len) d = (i + start)%nat.
+  Proof.
+    induction len; destruct i; intros; simpl; try lia.
+    rewrite IHlen; lia.
+  Qed.
+
+  Lemma nth_inj {A} n : forall (l l': list A) d,
+    length l = n ->
+    length l' = n ->
+    (forall i, (i < n)%nat -> nth i l d = nth i l' d) ->
+    l = l'.
+  Proof.
+    induction n; destruct l, l'; cbn [List.length]; intros * ?? Hi; try lia.
+    - reflexivity.
+    - f_equal.
+      + apply (Hi 0%nat ltac:(lia)).
+      + eapply IHn; eauto; intros i0 Hi0.
+        apply (Hi (S i0)%nat ltac:(lia)).
+  Qed.
+
+  Lemma nth_repeat {A} (a d: A): forall n i,
+      (i < n)%nat ->
+      nth i (repeat a n) d = a.
+  Proof.
+    induction n; destruct i; simpl; intros; try lia.
+    - reflexivity.
+    - apply IHn; lia.
+  Qed.
+
+  Lemma nth_repeat_default {A} (d: A): forall n i,
+      nth i (repeat d n) d = d.
+  Proof.
+    intros; destruct (Nat.lt_ge_cases i n).
+    - rewrite nth_repeat by lia; reflexivity.
+    - rewrite nth_overflow by (rewrite repeat_length; lia); reflexivity.
+  Qed.
+
+  Lemma map_seq_nth_slice {A} (l: list A) (d: A) :
+    forall len start,
+      List.map (fun idx => nth idx l d) (seq start len) =
+      List.firstn len (List.skipn start l) ++
+      repeat d (start + len - Nat.max start (List.length l)).
+  Proof.
+    intros.
+    eapply @nth_inj with (d := d); intros.
+    - rewrite map_length, seq_length; reflexivity.
+    - rewrite app_length, firstn_length, repeat_length, skipn_length; lia.
+    - destruct (Nat.lt_ge_cases i (List.length (List.firstn len (List.skipn start l))));
+        [rewrite app_nth1 by lia | rewrite app_nth2 by lia].
+      all: rewrite <- nth_nth_nth_map with (dn := List.length l) by lia.
+      all: rewrite nth_seq by lia.
+      + rewrite nth_firstn, nth_skipn by lia; reflexivity.
+      + rewrite firstn_length, skipn_length in *.
+        rewrite nth_overflow, nth_repeat_default by lia.
+        reflexivity.
+  Qed.
+
+  Lemma map_seq_nth_slice_le {A} (l: list A) (d: A) :
+    forall len start,
+      (start + len <= List.length l)%nat ->
+      List.map (fun idx => nth idx l d) (seq start len) =
+      List.firstn len (List.skipn start l).
+  Proof.
+    intros; rewrite map_seq_nth_slice.
+    replace (_ + _ - _)%nat with 0%nat by lia; simpl.
+    rewrite app_nil_r; reflexivity.
+  Qed.
+
+  Lemma le_combine_nth_chunk n (bs: list byte) idx dd:
+    n <> 0%nat ->
+    (idx < Nat.div_up (Datatypes.length bs) n)%nat ->
+    le_combine (nth idx (chunk n bs) dd) =
+    le_combine (List.map (fun idx => nth idx bs Byte.x00) (seq (idx * n) n)).
+  Proof.
+    intros.
+    rewrite nth_chunk by assumption.
+    rewrite map_seq_nth_slice, le_combine_app_0.
+    reflexivity.
+  Qed.
+
+  Lemma In_map_combine_in_bounds n (Hn: n <> 0%nat) bs a:
+    In a (List.map le_combine (chunk n bs)) ->
+    0 <= a < 2 ^ (8 * Z.of_nat n).
+  Proof.
+    intros; eapply (Forall_In (Forall_le_combine_in_bounds n bs ltac:(lia)));
+      eassumption.
+  Qed.
+
+  Lemma ip_checksum_impl_ok bs:
+    ip_checksum_impl bs = word.of_Z (ip_checksum bs).
+  Proof.
+    unfold ip_checksum, ip_checksum_impl, nlet, co_word_of_byte, co_word_of_Z.
+    rewrite ranged_for_all_nd_combine2 by lia.
+    rewrite <- fold_left_as_ranged_for_all_nd.
+    rewrite word.morph_and, word.morph_not.
+    erewrite fold_left_push_fn
+      with (f' := fun w z => word_onec_add16 w (word.of_Z z))
+           (P := fun x => in_bounds 16 x); cycle 1.
+    { intros.
+      eapply onec_add16_bounds; try eassumption.
+      eapply (In_map_combine_in_bounds 2); eassumption || lia. }
+    { intros * Hin%(In_map_combine_in_bounds 2 ltac:(lia)) Ha0.
+      eapply word_morph_onec_add; eassumption. }
+    { red; lia. }.
+    { rewrite (copying_fold_left_as_ranged_fold_left _ (List.map _ _)).
+      rewrite map_length, length_chunk by lia.
+      do 2 f_equal; apply fold_left_Proper; try reflexivity; []. {
+        intros * Hin%z_range_sound.
+        unfold ip_checksum_upd, nlet, co_word_of_byte, co_word_of_Z.
+        rewrite nth_error_nth' with (d := le_combine [default; default])
+          by (rewrite map_length, length_chunk; lia).
+        rewrite !map_nth, le_combine_nth_chunk by lia.
+        cbn [le_combine seq List.map].
+        rewrite word.morph_or, Z.lor_0_r, word.morph_shiftl by lia.
+        unfold word_onec_add16, ListArray.get, cast, Convertible_Z_nat.
+        repeat (lia || f_equal).
+      }
+    }
+  Qed.
+
+  Lemma ip_checksum_impl_ok' bs:
+    ip_checksum bs = word.unsigned (ip_checksum_impl bs).
+  Proof.
+    rewrite ip_checksum_impl_ok, word.unsigned_of_Z_nowrap.
+    - reflexivity.
+    - pose proof ip_checksum_bounds bs; lia.
+  Qed.
+End Properties.
